tactics: introduce __by_tactic
to be the actual tactics marker, taking an already-reified tactic

ulib/FStar.Tactics.Effect.fst
@@ -72,14 +72,16 @@ let reify_tactic (t:tactic 'a) : __tac 'a =
   fun s -> reify (t ()) s
 
 abstract
-let by_tactic (t:__tac 'a) (p:Type) : Type = p
+let __by_tactic (t:__tac 'a) (p:Type) : Type = p
+
+unfold let by_tactic (t : tactic 'a) (p:Type) : Type = __by_tactic (reify_tactic t) p
 
 // Must run with tactics off, as it will otherwise try to run `by_tactic
 // (reify_tactic t)`, which fails as `t` is not a concrete tactic
 #reset-options "--no_tactics"
 let assert_by_tactic (t:tactic 'a) (p:Type)
   : Pure unit
-         (requires (by_tactic (reify_tactic t) (squash p)))
+         (requires (by_tactic t (squash p)))
          (ensures (fun _ -> p))
   = ()
 #reset-options
